backend/Linear.v
@@ -239,6 +239,7 @@ Inductive step: state -> trace -> state -> Prop :=
       sig = funsig f' ->
       forall COMP: comp_of f' = comp_of f,
       forall (NOTEXT: forall ef, f' <> External ef),
+      forall (SIG_RES: sig_res sig = sig_res (parent_signature s)),
       Mem.free m stk 0 f.(fn_stacksize) (comp_of f) = Some m' ->
       step (State s f (Vptr stk Ptrofs.zero) (Ltailcall sig ros :: b) rs m)
         E0 (Callstate s f' sig rs' m' (comp_of f))
