backend/Tunnelingproof.v
@@ -756,6 +756,7 @@ Proof.
   apply sig_preserved.
   unfold tunnel_fundef. now rewrite comp_tunnel_fundef, comp_transl.
   destruct fd; simpl in *; try congruence.
+  inv STK; eauto. inv H; eauto.
   econstructor; eauto using return_regs_lessdef, match_parent_locset.
 - (* Lbuiltin *)
   exploit eval_builtin_args_lessdef. eexact LS. eauto. eauto. intros (tvargs & EVA & LDA).
